init0

share/pulse/examples/dice/dpe/SPDM3.fst
@@ -55,20 +55,14 @@ let init_inv (key_len:u32) (b:Seq.seq u8) (s:state) (r:gref) : slprop =
 
 let pcm_elt (p:perm) (t:trace) : pcm_t = Some p, t
 
-
 fn init0 (key_size:u32) (signing_pub_key:V.vec u8 { V.length signing_pub_key == U32.v key_size })
-  (#p:perm)
   (#s:Seq.seq u8)
-  requires V.pts_to signing_pub_key #p s
+  requires V.pts_to signing_pub_key s
   returns r:state & gref
-  ensures V.pts_to signing_pub_key #p s **
-          init_inv key_size s (fst r) (snd r)
+  ensures init_inv key_size s (fst r) (snd r)
 {
   let session_transcript = V.alloc 0uy 0sz;
   
-  //prove this assumption
-  _assume ((Seq.Base.create (SZ.v 0sz) 0uy) == Seq.empty);
-
   let st_repr = { key_size; signing_pub_key; session_transcript };
   let c_st = Initialized st_repr;
   
@@ -78,102 +72,19 @@ fn init0 (key_size:u32) (signing_pub_key:V.vec u8 { V.length signing_pub_key == 
   let trace = next_trace emp_trace tr_elt;
   
   let r = ghost_alloc #trace_pcm_t #trace_pcm (pcm_elt 1.0R trace);
-  
- (*Current context:
-    ghost_pcm_pts_to r (G.reveal (G.hide (pcm_elt 1.0R trace))) **
-    V.pts_to session_transcript (Seq.Base.create (SZ.v 0sz) 0uy) **
-    V.pts_to signing_pub_key s*)
-
-  
-  with _v. rewrite  (ghost_pcm_pts_to r (G.reveal (G.hide _v))) as 
-                     (ghost_pcm_pts_to r _v);
-  assert (pure (st_repr.key_size == repr.key_size_repr));
-  assert (V.pts_to session_transcript (Seq.Base.create (SZ.v 0sz) 0uy));
 
   rewrite each
-    signing_pub_key  as st_repr.signing_pub_key,
-    session_transcript as st_repr.session_transcript; 
-  
-  rewrite each 
-  s as repr.signing_pub_key_repr;
-  
-  rewrite each 
-  (Seq.Base.create (SZ.v 0sz) 0uy) as Seq.empty #u8;
+    signing_pub_key as st_repr.signing_pub_key,
+    s as repr.signing_pub_key_repr;
 
-  assert (pure (c_st == Initialized st_repr));
-  assert (pure (tr_elt == G_Initialized repr));
-  assert (pure (current_state trace == G_Initialized repr));
-  assert (V.pts_to st_repr.session_transcript Seq.Base.empty);
-  assert (pure (st_repr.key_size == repr.key_size_repr));
-  (*-----------------------------------------------------------------------------------*)
-  (*CONTEXT HAS THIS CONDITION, THEN WHY THE BELOW ASSERT IS NOT PASSING?*)
-  (*How can I add an assume, adding __assume with this condition shows some type error.*)
-  (*-----------------------------------------------------------------------------------*)
-  //assert ( V.pts_to st_repr.signing_pub_key repr.signing_pub_key_repr); //NEED TO UNDERSTAND THIS.
-  (*Current context:
-    ghost_pcm_pts_to r (pcm_elt 1.0R trace) **
-    V.pts_to st_repr.session_transcript Seq.Base.empty **
-    V.pts_to st_repr.signing_pub_key repr.signing_pub_key_repr*)
-  
-  match c_st {
-    Initialized st_repr -> {
-      //What is going wrong here? Why it is not typechecking or not showing errors?
-      //Plan is to say unreachable in all branches except the G_Initialized
-      show_proof_state;
-       (*match (current_state trace){
-        G_UnInitialized  -> {
-          admit()
-        }
-        G_Initialized _ -> {
-          admit()
-        }
-        G_Recv_no_sign_resp _ -> {
-          admit()
-        }
-        G_Recv_sign_resp _ -> {
-          admit()
-        }
-       }*)
-      
-
-     }
-    
-     Recv_no_sign_resp st_repr -> {
-      
-      unreachable ()
-     }
-  }
-  
-(* G_UnInitialized ->{
-        admit()
-      }
-      G_Initialized k ->{
-        admit()
-      }
-      G_Recv_no_sign_resp  _ -> {
-        admit()
-      }
-      G_Recv_sign_resp _ -> {
-        admit()
-      }*)
-
-  (*(SPDM3.Initialized st)
-      (SPDM3.G_Initialized repr) ->
-      (V.pts_to st.signing_pub_key repr.signing_pub_key_repr **
-      V.pts_to st.session_transcript Seq.Base.empty) **
-      pure (st.key_size == repr.key_size_repr)*)
-  
-  (* ghost_pcm_pts_to r (pcm_elt 1.0R trace) **
-    V.pts_to st_repr.session_transcript Seq.Base.empty **
-    V.pts_to st_repr.signing_pub_key repr.signing_pub_key_repr*)
-
-  (*To prove,
-    exists* (t:trace).
-    spdm_inv s r t ** 
-    pure (G_Initialized? (current_state t) /\
-          g_key_of_gst (current_state t) == b /\
-          g_key_len_of_gst (current_state t) == key_len)*)
-  
+  assert_ (pure (Seq.equal (Seq.create (SZ.v 0sz) 0uy) Seq.empty));
+  with _v. rewrite (V.pts_to session_transcript _v) as
+                   (V.pts_to st_repr.session_transcript Seq.empty);
+  fold (session_state_related (Initialized st_repr) (G_Initialized repr));
+  fold (spdm_inv c_st r trace);
+  let res = (Initialized st_repr, r);
+  fold (init_inv key_size s (fst res) (snd res));
+  res
 }
 
 (*rewrite each
